theories/lang.v
@@ -447,7 +447,7 @@ Fixpoint select u fv (query : Callable) (modes:list mode) (rules: list R) sigma 
 *)
 (*SNIP: bc_type*)
 Definition bc : Unif -> program -> fvS -> Callable -> 
-                        Sigma -> (fvS * seq (Sigma * R)) :=
+                        Sigma -> fvS * seq (Sigma * R) :=
 (*ENDSNIP: bc_type*)
   fun u pr fv (query:Callable) s =>
   match tm2RC (deref s (Callable2Tm query)) with
